\begin{figure}[!t]
  \centering
  \begin{subfigure}[b]{0.45\textwidth}
    \begin{lstlisting}[frame=tb, mathescape=true]
let rec sort$^o$ x y =
    (x === Nil /\ y === Nil) \/
    (fresh s, xs, xs$_1$ in
      (smallest$^o$ x s xs /\
       sort$^o$ xs xs$_1$ /\
       y === (s :: xs$_1$)))
let rec smallest$^o$ l s l$_1$ =
  (l === [s] /\ l$_1$ ===  Nil) \/
  (fresh  h, t, s$_1$, t$_1$, max in
      l === (h :: t) /\
      smallest$^o$ t s$_1$ t$_1$ /\
      minmax$^o$ h s$_1$ s max /\
      l$_1$ ===  (max :: t$_1$) 
    );
    \end{lstlisting}
   \caption{Implementation in \mk}
    \label{fig:sortIn}
  \end{subfigure}
  \hfill
  \begin{subfigure}[b]{0.45\textwidth}
    \begin{lstlisting}[frame=tb, mathescape=true]

let rec sort$^o$ x$^{f \rightarrow g}$ y$^{g \rightarrow g}$ =
    (x$^{f \rightarrow g}$ ===    Nil /\ y$^{g \rightarrow g}$ ===    Nil) \/
    (fresh s, xs, xs$_1$ in
      (y$^{g \rightarrow g}$ ===    (s$^{f \rightarrow g}$ :: xs$_1$$^{f \rightarrow g}$) /\
       Unfold sort$^o$ xs$^{f \rightarrow g}$ xs$_1$$^{g \rightarrow g}$ /\
       Unfold smallest$^o$ x$^{f \rightarrow g}$ s$^{g \rightarrow g}$ xs$^{g \rightarrow g}$))
let rec smallest$^o$ l$^{f \rightarrow g}$ s$^{g \rightarrow g}$ l$_1$$^{g \rightarrow g}$ =
  (l$^{f \rightarrow g}$ ===    [s$^{g \rightarrow g}$] /\ l$_1$$^{g \rightarrow g}$ ===       Nil) \/
  (fresh  h, t, s$_1$, t$_1$, max in
      l$_1$$^{g \rightarrow g}$ ===     (max$^{f \rightarrow g}$ :: t$_1$$^{f \rightarrow g}$) /\
      Unfold minmax$^o$ h$^{f \rightarrow g}$ s$_1$$^{f \rightarrow g}$ s$^{g \rightarrow g}$ max$^{g \rightarrow g}$ /\
      Unfold smallest$^o$ t$^{f \rightarrow g}$ s$_1$$^{g \rightarrow g}$ t$_1$$^{g \rightarrow g}$ /\
      l$^{f \rightarrow g}$ ===    (h$^{g \rightarrow g}$ :: t$^{g \rightarrow g}$) 
    );
    \end{lstlisting}
    \caption{Mode inference and Binding time analysis result}
    \label{fig:sortModded}
  \end{subfigure}

  \hfill

  \begin{subfigure}[b]{0.45\textwidth}
    \begin{lstlisting}[frame=tb, mathescape=true]
let sort$^o$ y0 =
  (y0 === (O :: (S (O) :: 
    [S (S (O))])) \/
   y0 === (O :: (S (S (O))
    :: [S (O)])) \/
   y0 === (S (O) :: 
    (Zero :: [S (S (O))])) ...
   
    \end{lstlisting}
    \caption{Conjunction Partial Deduction result}
    \label{fig:sortDeduced}
  \end{subfigure}
\hfill
  \begin{subfigure}[b]{0.45\textwidth}
    \begin{lstlisting}[frame=tb, mathescape=true]
sortoO = msum 
    [do { let {x1 = Zero}
        ; let {x4 = Zero}
        ; let {x3 = Succ x4}
        ; let {x8 = Zero}
        ...
        ; let {x0 = Cons x15 x16}
        ; return x0},...
    \end{lstlisting}
    \caption{Functional conversion into \haskell}
    \label{fig:sortHaskell}
  \end{subfigure}

  \caption{Multiplication relation}
  \label{fig:sort}
\end{figure}